{
 "cells": [
  {
   "cell_type": "markdown",
   "id": "7be059af-1529-447b-b93a-d2f186b41af1",
   "metadata": {},
   "source": [
    "# Questions:\n",
    "---\n",
    "\n",
    "1. $\\textbf{Why do we need to prove?}$\n",
    "\n",
    "    We need to prove to ensure the accuracy and reliability of statements or theorems, providing a solid foundation for further reasoning and problem-solving.\n",
    "    \n",
    "2. $\\textbf{If we fail to generate a proof, what will happen?}$\n",
    "\n",
    "    If we fail to generate a proof, the statement or theorem remains unverified and cannot be accepted as true. This lack of proof prevents it from being used reliably in further mathematical reasoning or applications, potentially leading to errors and incorrect conclusions."
   ]
  },
  {
   "cell_type": "markdown",
   "id": "879c4112-4a6e-4de5-b189-10883ed2e140",
   "metadata": {},
   "source": [
    "# Exercises:\n",
    "---\n",
    "1. $\\textbf{Is the number 0 even or odd?}$\n",
    "\n",
    "    Express 0 as 2k, where k = 0:\n",
    "   \n",
    "    2(0) = 2 × 0\n",
    "\n",
    "     Since 0 can be expressed in the form 2k, where k is an integer, we can conclude    that 0 is an $\\textbf{even}$ number.\n",
    "\n",
    "\n",
    "\n",
    "\n",
    "3. $\\textbf{Is the number -301 even or odd?}$\n",
    "\n",
    "    Express -301 as 2k+1, where k = -301:\n",
    "   \n",
    "   -301 = 2k + 1\n",
    "\n",
    "   k = -151\n",
    "\n",
    "   Since k is an integer, we can express -301 in the form of 2k+1, where k = -151, therefore the number -301 is $\\textbf{odd.}$\n",
    "\n",
    "5. $\\textbf{If a and b are integers, is the expression $6a^2b$ even or odd?}$\n",
    "\n",
    "   Rewrite the expression as a product of its factors:\n",
    "   $6a^2b$ = 2 × 3 × $a^2$ × b\n",
    "\n",
    "      Consider the factors individually:\n",
    "   - 2 is an even number.\n",
    "   - 3 is an odd number.\n",
    "   - $a^2$ is even, as any integer raised to an even power is even.\n",
    "   - b can be either even or odd.\n",
    "  \n",
    "     \n",
    "   Since we have a product of even (2 and $a^2$) and possibly odd (3 and b) factors, the overall expression will be even.\n",
    "\n",
    "    Therefore, the expression $6a^2b$ is $\\textbf{even}$, assuming that a and b are integers.\n",
    "   \n",
    "5. $\\textbf{If a and b are integers, is the expression $10a+8b+1$ even or odd?}$\n",
    "\n",
    "    Break down the expression and consider the even or odd nature of each term:\n",
    "   - 10a is even, being a multiple of 10 (an even number).\n",
    "   - 8b is even, being a multiple of 8 (an even number).\n",
    "   - 1 is odd.\n",
    "\n",
    "    Consider the sum of these terms:\n",
    "   10a (even) + 8b (even) + 1 (odd)\n",
    "\n",
    "    When we add an even number (10a) and another even number (8b) to an odd number (1), the result is an odd number. This is because the sum of any two even numbers is always even, and adding an odd number to an even number results in an odd number.\n",
    "\n",
    "    Therefore, the expression 10a + 8b + 1 is $\\textbf{odd}$, assuming that a and b are integers."
   ]
  },
  {
   "cell_type": "markdown",
   "id": "d676c15f-b36a-4928-9157-3cc409ffb271",
   "metadata": {},
   "source": [
    "1. $\\textbf{List down the first 6 prime numbers:}$\n",
    "2, 3, 5, 7, 11, 13\n",
    "\n",
    "2. $\\textbf{List down the first 6 composite numbers:}$\n",
    "4, 6, 8, 9, 10, 11\n"
   ]
  },
  {
   "cell_type": "markdown",
   "id": "fd8bd31b-e7f7-4385-a32e-1d308b314c3c",
   "metadata": {},
   "source": [
    "# 1. Prove that the Euler's number $e = \\Sigma_{k=0}^\\infty \\frac{1}{k!} \\notin \\mathbb{Q}$.\n",
    "---\n",
    "Recall that a rational number is one that can be expressed as the quotient of two integers. We want to prove that Euler's number $e = \\sum_{k=0}^\\infty \\frac{1}{k!} \\notin \\mathbb{Q}$.\n",
    "\n",
    "Suppose that there is a reasonable contradictiononal, then $e = \\frac{a}{b}$, where $a$ and $b$ are integers and $b \\neq 0$.\n",
    "\n",
    "Consider the series expansion of $e$:\n",
    "\n",
    "\\[ $e = \\sum_{k=0}^\\infty \\frac{1}{k!} = 1 + \\frac{1}{1!} + \\frac{1}{2!} + \\frac{1}{3!} + \\dots $\\]\n",
    "\n",
    "Multiply both sides by $b!$ to clear the denominators:\n",
    "\n",
    "\\[ $b!e = b!\\left(1 + \\frac{1}{1!} + \\frac{1}{2!} + \\frac{1}{3!} + \\dots \\right) = b!(1 + b + \\frac{b(b-1)}{2!} + \\frac{b(b-1)(b-2)}{3!} + \\dots)$ \n",
    "\n",
    "Now, note that each term is a multiple of $b!$, hence the right side is an integer. Thus, $e$ must be rational, contradicting our assumption. Therefore, we can now conclude that $e \\notin \\mathbb{Q}$."
   ]
  },
  {
   "cell_type": "markdown",
   "id": "a0562f30",
   "metadata": {},
   "source": [
    "# 2. Prove Minkowski's Inequality for sums, $\\forall \\ p>1, (a_k, b_k)>0$:\n",
    "---\n",
    "\n",
    "We want to prove Minkowski's Inequality for sums:\n",
    "\\[ $\\left(\\sum_{k=1}^n |a_k + b_k|^p\\right)^\\frac{1}{p} \\leq \\left(\\sum_{k=1}^n |a_k|^p\\right)^\\frac{1}{p} + \\left(\\sum_{k=1}^n |b_k|^p\\right)^\\frac{1}{p} $\\]\n",
    "\n",
    "$\\textit{Proof:}$\n",
    "\n",
    "The proof involves using Hölder's inequality. Let $q$ be the conjugate exponent of $p$ (i.e., $\\frac{1}{p} + \\frac{1}{q} = 1$).\n",
    "\n",
    "Apply Hölder's inequality with $p$ and $q$ to the sequences $(|a_k|^p)$ and $(1)$, and to the sequences $(|b_k|^p)$ and $(1)$:\n",
    "\n",
    "\\[ $\\sum_{k=1}^n |a_k|^p \\cdot 1 \\leq \\left(\\sum_{k=1}^n |a_k|^p\\right)^\\frac{1}{p} \\left(\\sum_{k=1}^n 1^q\\right)^\\frac{1}{q} = \\left(\\sum_{k=1}^n |a_k|^p\\right)^\\frac{1}{p} \\cdot n^\\frac{1}{q} $\\]\n",
    "\\[ $\\sum_{k=1}^n |b_k|^p \\cdot 1 \\leq \\left(\\sum_{k=1}^n |b_k|^p\\right)^\\frac{1}{p} \\left(\\sum_{k=1}^n 1^q\\right)^\\frac{1}{q} = \\left(\\sum_{k=1}^n |b_k|^p\\right)^\\frac{1}{p} \\cdot n^\\frac{1}{q} $\\]\n",
    "\n",
    "Add these inequalities:\n",
    "\n",
    "\\[ $\\sum_{k=1}^n |a_k|^p + \\sum_{k=1}^n |b_k|^p \\leq \\left(\\sum_{k=1}^n |a_k|^p\\right)^\\frac{1}{p} \\cdot n^\\frac{1}{q} + \\left(\\sum_{k=1}^n |b_k|^p\\right)^\\frac{1}{p} \\cdot n^\\frac{1}{q} $\\]\n",
    "\n",
    "\\[ $\\sum_{k=1}^n (|a_k|^p + |b_k|^p) \\leq \\left(\\sum_{k=1}^n |a_k|^p\\right)^\\frac{1}{p} \\cdot n^\\frac{1}{q} + \\left(\\sum_{k=1}^n |b_k|^p\\right)^\\frac{1}{p} \\cdot n^\\frac{1}{q} $\\]\n",
    "\n",
    "Now, raise both sides to the power of $\\frac{1}{p}$:\n",
    "\n",
    "\\[ $\\left(\\sum_{k=1}^n (|a_k|^p + |b_k|^p)\\right)^\\frac{1}{p} \\leq \\left(\\left(\\sum_{k=1}^n |a_k|^p\\right)^\\frac{1}{p} \\cdot n^\\frac{1}{q} + \\left(\\sum_{k=1}^n |b_k|^p\\right)^\\frac{1}{p} \\cdot n^\\frac{1}{q}\\right)^\\frac{1}{p} $\\]\n",
    "\n",
    "\\[ $\\left(\\sum_{k=1}^n (|a_k + b_k|^p)\\right)^\\frac{1}{p} \\leq \\left(\\sum_{k=1}^n |a_k|^p\\right)^\\frac{1}{p} + \\left(\\sum_{k=1}^n |b_k|^p\\right)^\\frac{1}{p} $\\]\n",
    "\n",
    "Which proves Minkowski's Inequality."
   ]
  },
  {
   "cell_type": "markdown",
   "id": "22644aad",
   "metadata": {},
   "source": [
    "# 3. Prove the triangle inequality $|x+y| \\leq |x| + |y|, \\forall (x,y) \\in \\mathbb{R}$\n",
    "---\n",
    "\n",
    "$\\textit{Proof:}$\n",
    "\n",
    "Consider three cases:\n",
    "\n",
    "1. If $x \\geq 0$ and $y \\geq 0$, then $|x| = x$ and $|y| = y$, so $|x+y| = x+y$. Then $|x+y| = x + y \\leq |x| + |y|$.\n",
    "2. If $x \\geq 0$ and $y < 0$, then $|x| = x$ and $|y| = -y$, so $|x+y| = x-y$. Then $|x+y| = x - y \\leq |x| + |y|$.\n",
    "3. If $x < 0$ and $y < 0$, then $|x| = -x$ and $|y| = -y$, so $|x+y| = -(x+y) = -x - y$. Then $|x+y| = -(x + y) \\leq |x| + |y|$."
   ]
  },
  {
   "cell_type": "markdown",
   "id": "08381626",
   "metadata": {},
   "source": [
    "# 4. Prove Sedrakayan's Lemma $\\forall u_i, v_i \\in \\mathbb{R}^+$:\n",
    "---\n",
    "\n",
    "Prove Sedrakayan's Lemma $\\forall u_i, v_i \\in \\mathbb{R}^+$:\n",
    "\n",
    "$\\frac{(\\sum_{i=1}^n u_i)^2}{\\sum_{i=1}^n v_i} \\leq \\sum_{i=1}^n \\frac{(u_i)^2}{v_i}$\n",
    "\n",
    "$\\textit{Proof:}$\n",
    "\n",
    "Let $\\mathbf{u} = (u_1, u_2, ..., u_n)$ and $\\mathbf{v} = (v_1, v_2, ..., v_n)$ be vectors in $\\mathbb{R}^+$.\n",
    "\n",
    "By Cauchy-Schwarz Inequality, we have:\n",
    "\n",
    "$\\left(\\sum_{i=1}^n u_i v_i\\right)^2 \\leq \\left(\\sum_{i=1}^n u_i^2\\right) \\left(\\sum_{i=1}^n v_i^2\\right)$\n",
    "\n",
    "Since $v_i > 0$ for all $i$, we can divide both sides by $\\left(\\sum_{i=1}^n v_i^2\\right): \\frac{\\left(\\sum_{i=1}^n u_i v_i\\right)^2}{\\left(\\sum_{i=1}^n v_i^2\\right)} \\leq \\sum_{i=1}^n u_i^2$\n",
    "\n",
    "Now, notice that $\\left(\\sum_{i=1}^n u_i v_i\\right) = \\mathbf{u} \\cdot \\mathbf{v}$ and $\\sum_{i=1}^n u_i^2 = \\|\\mathbf{u}\\|^2$, where $\\|\\cdot\\|$ denotes the Euclidean norm.\n",
    "\n",
    "Thus, we have: $\\frac{(\\mathbf{u} \\cdot \\mathbf{v})^2}{\\|\\mathbf{v}\\|^2} \\leq \\|\\mathbf{u}\\|^2$\n",
    "\n",
    "Dividing both sides by $\\|\\mathbf{v}\\|^2$, we get: $\\frac{(\\mathbf{u} \\cdot \\mathbf{v})^2}{\\|\\mathbf{v}\\|^2 \\|\\mathbf{v}\\|^2} \\leq \\frac{\\|\\mathbf{u}\\|^2}{\\|\\mathbf{v}\\|^2}$\n",
    "\n",
    "Simplifying, we obtain: $\\frac{(\\mathbf{u} \\cdot \\mathbf{v})^2}{\\|\\mathbf{v}\\|^4} \\leq \\frac{\\|\\mathbf{u}\\|^2}{\\|\\mathbf{v}\\|^2}$\n",
    "\n",
    "Now, substituting $\\|\\mathbf{v}\\|^2 = \\sum_{i=1}^n v_i$ and rearranging, we get: $\\frac{(\\sum_{i=1}^n u_i)^2}{\\sum_{i=1}^n v_i} \\leq \\sum_{i=1}^n \\frac{u_i^2}{v_i}$\n",
    "\n",
    "This proves Sedrakayan's Lemma.\n",
    "\n"
   ]
  },
  {
   "cell_type": "markdown",
   "id": "f55dfce8",
   "metadata": {},
   "source": [
    "# 5. Consider the functions $f(x) = 2x+1$, $g(x)=2y-1$, $j(x) = |f(x)+g(x)|$, and $h(x) = j(x)^2$, show for the following inequality that: $\\sqrt{|f(x)|^2} \\geq \\sqrt{h(x)} - \\sqrt{|g(x)|^2}, \\forall (x,y) \\in \\mathbb{Z}^+$\n",
    "---\n",
    "\n",
    "$\\textit{Proof:}$\n",
    "\n",
    "First, let's express $f(x)$, $g(x)$, and $h(x)$ in terms of $x$ and $y$:\n",
    "\n",
    "$f(x) = 2x + 1$\n",
    "\n",
    "$g(x) = 2y - 1$\n",
    "\n",
    "$j(x) = |f(x) + g(x)| = |(2x + 1) + (2y - 1)| = |2x + 2y| = 2|x + y|$\n",
    "\n",
    "$h(x) = j(x)^2 = (2|x + y|)^2 = 4|x + y|^2$\n",
    "\n",
    "Now, let's substitute $f(x)$, $g(x)$, and $h(x)$ back into the inequality:\n",
    "\n",
    "$\\sqrt{|(2x + 1)|^2} \\geq \\sqrt{(4|x + y|^2)} - \\sqrt{|(2y - 1)|^2}$\n",
    "\n",
    "Simplify each term:\n",
    "\n",
    "$\\sqrt{(2x + 1)^2} \\geq \\sqrt{4(|x + y|^2)} - \\sqrt{(2y - 1)^2}$\n",
    "\n",
    "$|2x + 1| \\geq 2|x + y| - |2y - 1|$\n",
    "\n",
    "Now, let's consider the absolute value expressions:\n",
    "\n",
    "1. $|2x + 1| = \\begin{cases} 2x + 1, & \\text{if } 2x + 1 \\geq 0 \\\\ -(2x + 1), & \\text{if } 2x + 1 < 0 \\end{cases}$\n",
    "2. $|2y - 1| = \\begin{cases} 2y - 1, & \\text{if } 2y - 1 \\geq 0 \\\\ -(2y - 1), & \\text{if } 2y - 1 < 0 \\end{cases}$\n",
    "\n",
    "Given that $x$ and $y$ are positive integers, both $2x + 1$ and $2y - 1$ are non-negative.\n",
    "\n",
    "Substitute back into the inequality:\n",
    "\n",
    "$2x + 1 \\geq 2|x + y| - (2y - 1)$\n",
    "\n",
    "$2x + 1 \\geq 2x + 2y - 2y + 1$\n",
    "\n",
    "$2x + 1 \\geq 2x + 1$\n",
    "\n",
    "This inequality holds true for all positive integers $x$ and $y$. Therefore, the inequality is true.\n",
    "\n",
    "Hence, we have shown that: $\\sqrt{|f(x)|^2} \\geq \\sqrt{h(x)} - \\sqrt{|g(x)|^2}, \\forall (x,y) \\in \\mathbb{Z}^+$"
   ]
  },
  {
   "cell_type": "markdown",
   "id": "05026e7c",
   "metadata": {},
   "source": [
    "# 6. Prove Sedrakayan's Lemma if $u_i, v_i$ are square roots of an even integers: $\\frac{(\\Sigma_{i=1}^n u_i)^2}{\\Sigma_{i=1}^n v_i}\\leq\\Sigma_{i=1}^n \\frac{(u_i)^2}{v_i}$\n",
    "---\n",
    "\n",
    "$\\textit{Proof:}$\n",
    "\n",
    "Let $u_i = \\sqrt{2x_i}$ and $v_i = \\sqrt{2y_i}$, where $x_i$ and $y_i$ are positive integers.\n",
    "\n",
    "Substitute $u_i$ and $v_i$ into the inequality:\n",
    "\n",
    "$\\frac{\\left(\\sum_{i=1}^n \\sqrt{2x_i}\\right)^2}{\\sum_{i=1}^n \\sqrt{2y_i}} \\leq \\sum_{i=1}^n \\frac{(\\sqrt{2x_i})^2}{\\sqrt{2y_i}}$\n",
    "\n",
    "$\\frac{\\left(\\sum_{i=1}^n \\sqrt{2x_i}\\right)^2}{\\sum_{i=1}^n \\sqrt{2y_i}} \\leq \\sum_{i=1}^n \\frac{2x_i}{\\sqrt{2y_i}}$\n",
    "\n",
    "Now, let's show that for any positive real numbers $a_i$ and $b_i$, we have:\n",
    "\n",
    "$\\left(\\sum_{i=1}^n a_i\\right)^2 \\leq n \\sum_{i=1}^n b_i$\n",
    "\n",
    "This is equivalent to:\n",
    "\n",
    "$\\left(\\sum_{i=1}^n a_i\\right)^2 \\leq \\sum_{i=1}^n (b_i)^2$\n",
    "\n",
    "which is a well-known result from the Cauchy-Schwarz Inequality.\n",
    "\n",
    "Substitute $a_i = \\sqrt{2x_i}$ and $b_i = \\frac{\\sqrt{2y_i}}{\\sqrt{n}}$ into the inequality:\n",
    "\n",
    "$\\left(\\sum_{i=1}^n \\sqrt{2x_i}\\right)^2 \\leq n \\sum_{i=1}^n \\left(\\frac{\\sqrt{2y_i}}{\\sqrt{n}}\\right)^2$\n",
    "\n",
    "$\\left(\\sum_{i=1}^n \\sqrt{2x_i}\\right)^2 \\leq \\sum_{i=1}^n 2y_i$\n",
    "\n",
    "Now, let's substitute this result back into our inequality:\n",
    "\n",
    "$\\frac{\\left(\\sum_{i=1}^n \\sqrt{2x_i}\\right)^2}{\\sum_{i=1}^n \\sqrt{2y_i}} \\leq \\sum_{i=1}^n \\frac{2x_i}{\\sqrt{2y_i}}$\n",
    "\n",
    "$\\frac{\\sum_{i=1}^n 2x_i}{\\sum_{i=1}^n \\sqrt{2y_i}} \\leq \\sum_{i=1}^n \\frac{2x_i}{\\sqrt{2y_i}}$\n",
    "\n",
    "$\\frac{\\sum_{i=1}^n 2x_i}{\\sum_{i=1}^n \\sqrt{2y_i}} \\leq \\sum_{i=1}^n \\frac{2x_i}{\\sqrt{2y_i}}$\n",
    "\n",
    "Since both sides are non-negative, we can square both sides of the inequality:\n",
    "\n",
    "$\\left(\\frac{\\sum_{i=1}^n 2x_i}{\\sum_{i=1}^n \\sqrt{2y_i}}\\right)^2 \\leq \\left(\\sum_{i=1}^n \\frac{2x_i}{\\sqrt{2y_i}}\\right)^2$\n",
    "\n",
    "$\\frac{\\left(\\sum_{i=1}^n 2x_i\\right)^2}{\\left(\\sum_{i=1}^n \\sqrt{2y_i}\\right)^2} \\leq \\sum_{i=1}^n \\frac{4x_i^2}{2y_i}$\n",
    "\n",
    "$\\frac{\\left(\\sum_{i=1}^n 2x_i\\right)^2}{\\sum_{i=1}^n 2y_i} \\leq \\sum_{i=1}^n \\frac{2x_i^2}{y_i}$\n",
    "\n",
    "$\\frac{\\left(\\sum_{i=1}^n u_i\\right)^2}{\\sum_{i=1}^n v_i} \\leq \\sum_{i=1}^n \\frac{(u_i)^2}{v_i}$\n",
    "\n",
    "This proves Sedrakayan's Lemma when $u_i$ and $v_i$ are square roots of even integers.\n"
   ]
  }
 ],
 "metadata": {
  "kernelspec": {
   "display_name": "Python 3 (ipykernel)",
   "language": "python",
   "name": "python3"
  },
  "language_info": {
   "codemirror_mode": {
    "name": "ipython",
    "version": 3
   },
   "file_extension": ".py",
   "mimetype": "text/x-python",
   "name": "python",
   "nbconvert_exporter": "python",
   "pygments_lexer": "ipython3",
   "version": "3.10.10"
  }
 },
 "nbformat": 4,
 "nbformat_minor": 5
}
